Finish local trace semantics. Fix makefile.

HoareLogic/Trace.v
@@ -1,4 +1,5 @@
 Require Import Coq.Relations.Relation_Operators.
+Require Import Coq.Sets.Ensembles.
 Require Import Logic.lib.Stream.SigStream.
 Require Import Logic.lib.Stream.StreamFunctions.
 Require Import Logic.PropositionalLogic.KripkeSemantics.
@@ -21,30 +22,80 @@ Definition end_state {state: Type} (tr: trace state) (ms: MetaState state): Prop
   (is_inf_stream tr /\ ms = NonTerminating) \/
   (exists n ms', is_n_stream (S n) tr /\ tr n = Some (ms', ms)).
 
-Definition traces_app {state: Type} (d1 d2: trace state -> Prop): trace state -> Prop :=
+Definition traces (state: Type): Type := Ensemble (trace state).
+
+Definition traces_app {state: Type} (d1 d2: traces state): traces state :=
   fun tr =>
     (exists tr1 tr2, d1 tr1 /\ d2 tr2 /\ tr = stream_app tr1 tr2) \/
     (exists tr1, d1 tr1 /\ (end_state tr1 NonTerminating \/ end_state tr1 Error) /\ tr = tr1).
 
-Fixpoint traces_power {state: Type} (d: trace state -> Prop) (n: nat): trace state -> Prop :=
+Fixpoint traces_power {state: Type} (d: traces state) (n: nat): traces state :=
   match n with
   | 0 => is_empty_stream
   | S n => traces_app (traces_power d n) d
   end.
 
-Definition traces_pstar {state: Type} (d: trace state -> Prop): trace state -> Prop :=
+Definition traces_pstar {state: Type} (d: traces state): traces state :=
   fun tr => exists n, traces_power d n tr.
 
-Definition traces_pomega {state: Type} (d: trace state -> Prop): trace state -> Prop :=
+Definition traces_pomega {state: Type} (d: traces state): traces state :=
   fun tr => exists f, tr = stream_capp f /\ forall n, d (f n).
+
+Lemma traces_app_mono {state: Type}: forall (d1 d2 d3 d4: traces state),
+  Included _ d1 d3 ->
+  Included _ d2 d4 ->
+  Included _ (traces_app d1 d2) (traces_app d3 d4).
+Proof.
+  intros.
+  unfold Included, Ensembles.In in *; intros tr ?.
+  destruct H1.
+  + destruct H1 as [tr1 [tr2 [? [? ?]]]].
+    left; exists tr1, tr2; auto.
+  + destruct H1 as [tr1 [? [? ?]]].
+    right; exists tr1; auto.
+Qed.
+
+Lemma traces_power_mono {state: Type}: forall (d1 d2: traces state) (n: nat),
+  Included _ d1 d2 ->
+  Included _ (traces_power d1 n) (traces_power d2 n).
+Proof.
+  intros.
+  induction n.
+  + hnf; intros; auto.
+  + simpl.
+    apply traces_app_mono; auto.
+Qed.
+
+Lemma traces_pstar_mono {state: Type}: forall (d1 d2: traces state),
+  Included _ d1 d2 ->
+  Included _ (traces_pstar d1) (traces_pstar d2).
+Proof.
+  intros.
+  unfold Included, Ensembles.In; intros tr ?.
+  destruct H0 as [n ?].
+  exists n.
+  revert tr H0.
+  apply traces_power_mono; auto.
+Qed.
+
+Lemma traces_pomega_mono {state: Type}: forall (d1 d2: traces state),
+  Included _ d1 d2 ->
+  Included _ (traces_pomega d1) (traces_pomega d2).
+Proof.
+  intros.
+  unfold Included, Ensembles.In; intros tr ?.
+  destruct H0 as [f [? ?]].
+  exists f; split; auto.
+  intros; apply H, H1.
+Qed.
 
 Module Type DECREASE_TRACE.
 
 Declare Module D: DECREASE.
 
-Parameter decrease_trace: forall {state: Type} {kiM: KripkeIntuitionisticModel state}, trace state -> Prop.
+Parameter decrease_trace: forall {state: Type} {kiM: KripkeIntuitionisticModel state}, traces state.
 
-Parameter decrease_trace_with_test: forall {state: Type} {kiM: KripkeIntuitionisticModel state} (P: state -> Prop), trace state -> Prop.
+Parameter decrease_trace_with_test: forall {state: Type} {kiM: KripkeIntuitionisticModel state} (P: state -> Prop), traces state.
 
 End DECREASE_TRACE.
 
@@ -53,10 +104,10 @@ Module DecreaseTrace (D: DECREASE) <: DECREASE_TRACE with Module D := D.
 Module D := D.
 Export D.
 
-Definition decrease_trace {state: Type} {kiM: KripkeIntuitionisticModel state}: trace state -> Prop :=
+Definition decrease_trace {state: Type} {kiM: KripkeIntuitionisticModel state}: traces state :=
   fun tr => is_fin_stream tr /\ forall n ms ms', tr n = Some (ms, ms') -> decrease ms ms'.
 
-Definition decrease_trace_with_test {state: Type} {kiM: KripkeIntuitionisticModel state} (P: state -> Prop) : trace state -> Prop :=
+Definition decrease_trace_with_test {state: Type} {kiM: KripkeIntuitionisticModel state} (P: state -> Prop) : traces state :=
   fun tr => decrease_trace tr /\ exists ms, begin_state tr ms /\
     match ms with
     | Terminating s => P s
@@ -67,3 +118,29 @@ End DecreaseTrace.
 
 Module Partial := DecreaseTrace (ProgramState.Partial).
 Module Total := DecreaseTrace (ProgramState.Total).
+
+Lemma Total2Partial_decrease_trace
+      {state: Type}
+      {kiM: KripkeIntuitionisticModel state}:
+  Included _ Total.decrease_trace Partial.decrease_trace.
+Proof.
+  unfold Included, Ensembles.In; intros tr ?.
+  destruct H as [? ?].
+  split; auto.
+  intros.
+  apply Total2Partial_decrease, (H0 n); auto.
+Qed.
+
+Lemma Total2Partial_decrease_trace_with_test
+      {state: Type}
+      {kiM: KripkeIntuitionisticModel state}
+      (P: state -> Prop):
+  Included _
+   (Total.decrease_trace_with_test P)
+   (Partial.decrease_trace_with_test P).
+Proof.
+  unfold Included, Ensembles.In; intros tr ?.
+  destruct H as [? ?].
+  split; auto.
+  apply Total2Partial_decrease_trace; auto.
+Qed.
